fairis/heap_lang/examples/even_odd/interface.v
@@ -11,21 +11,29 @@ Inductive PubA := step_sync (k: nat).
 Global Instance PubA_EqDec: EqDecision PubA.
 Proof.
   intros [x] [y]. destruct (decide (x = y)); [left | right]; set_solver.
-Qed. 
+Qed.
 
-(* constructs an ActionModel with pre-defined set of public roles *)
-Definition BuildSubModel (St Priv Role: Type) Trans := {|
-   amSt := St;
-   amA := PubA + Priv;
-   amRole := Role;
-   amTrans := Trans;
-|}.
+Global Instance PubA_Cnt: Countable PubA.
+Proof.
+  eapply inj_countable with (f := fun x => match x with | step_sync k => k end).
+  intros. destruct x; reflexivity. 
+Qed.
 
-(* Convention: if the type of ActionModel's actions is defined as a sum,
-   the left summand defines "public" actions (used for synchronization)
-   and the right one defines "private" actions *)
-Definition pub_act {A B: Type} := @inl A B.
-Definition priv_act {A B: Type} := @inr A B.
+
+(* (* constructs an ActionModel with pre-defined set of public roles *) *)
+(* Definition BuildSubModel (St Priv Role: Type) Trans := {| *)
+(*    amSt := St; *)
+(*    amA := PubA + Priv; *)
+(*    amRole := Role; *)
+(*    amTrans := Trans; *)
+(* |}. *)
+
+
+(* (* convention: if the type of ActionModel's actions is defined as a sum, *)
+(*    the left summand defines "public" actions (used for synchronization) *)
+(*    and the right one defines "private" actions *) *)
+(* Definition pub_act {A B: Type} := @inl A B. *)
+(* Definition priv_act {A B: Type} := @inr A B. *)
 
 
 Class ActionModelExtra (AM: ActionModel) := {
@@ -42,15 +50,17 @@ Class ActionModelExtra (AM: ActionModel) := {
 
 
 Record EvenModel := {
-    eSt: Type;
-    ePriv: Type;
-    eRole: Type;
-    eTrans;
+    (* eSt: Type; *)
+    (* ePriv: Type; *)
+    (* eRole: Type; *)
+    (* eTrans; *)
 
-    cur_even: eSt -> nat;
 
-    even_AM := BuildSubModel eSt ePriv eRole eTrans;
+    (* even_AM := BuildSubModel eSt ePriv eRole eTrans; *)
+    even_AM: ActionModel; 
     even_AME :> ActionModelExtra even_AM;
+
+    cur_even: amSt even_AM -> nat;
 
     even_step_inv st st' k ρ
       (STEP: amTrans even_AM st (pub_act (step_sync k), Some ρ) st'):
@@ -59,7 +69,8 @@ Record EvenModel := {
       (STEP: amTrans even_AM st (pub_act (step_sync k), None) st'):
       cur_even st = k /\ cur_even st' = k + 1 /\ Nat.odd k;
     even_stutter_inv st st' a ρ
-      (STEP: amTrans even_AM st (priv_act a, Some ρ) st'):
+      (PRIV: a ∉ pub_actions)
+      (STEP: amTrans even_AM st (a, Some ρ) st'):
       cur_even st = cur_even st' (* /\ Nat.odd (cur_even st) *);
 
     ρ__e: amRole even_AM;
@@ -68,7 +79,7 @@ Record EvenModel := {
     even_syncable st (ODD: Nat.odd (cur_even st)):
       exists st', amTrans even_AM st (pub_act (step_sync (cur_even st)), None) st';
     even_stutterable st (ODD: Nat.odd (cur_even st)):
-      exists st' a, amTrans even_AM st (priv_act a, Some ρ__e) st';
+      exists st' a, a ∉ pub_actions /\ amTrans even_AM st (a, Some ρ__e) st';
 
     even_step_lr_nonincr st st' a oρ
       (STEP: amTrans even_AM st (a, oρ) st'):
@@ -81,30 +92,27 @@ Record EvenModel := {
   (* TODO: ? replace with "private actions don't preempt the sync one forever" condition *)
   even_pub_priv_disj (st__e: amSt even_AM):
     (exists k st__e', amTrans _ st__e (pub_act $ step_sync k, Some ρ__e) st__e') ->
-    (exists a st__e', amTrans _ st__e (priv_act a, Some ρ__e) st__e') ->
+    (exists a st__e', a ∉ pub_actions /\ amTrans _ st__e (a, Some ρ__e) st__e') ->
     False;
 }.
 
 
 Record OddModel := {
-    oSt: Type;
-    oPriv: Type;
-    oRole: Type;
-    oTrans;
-
-    cur_odd: oSt -> nat;
-
-    odd_AM := BuildSubModel oSt oPriv oRole oTrans;
+    (* odd_AM := BuildSubModel oSt oPriv oRole oTrans; *)
+    odd_AM: ActionModel;
     odd_AME :> ActionModelExtra odd_AM;
+
+    cur_odd: amSt odd_AM -> nat;
 
     odd_step_inv st st' k ρ
       (STEP: amTrans odd_AM st (pub_act (step_sync k), Some ρ) st'):
       cur_odd st = k /\ cur_odd st' = k + 1 /\ Nat.odd k;
     odd_sync_inv st st' k
-      (STEP: amTrans odd_AM st (inl (step_sync k), None) st'):
+      (STEP: amTrans odd_AM st (pub_act (step_sync k), None) st'):
       cur_odd st = k /\ cur_odd st' = k + 1 /\ Nat.even k;
     odd_stutter_inv st st' a ρ
-      (STEP: amTrans odd_AM st (priv_act a, Some ρ) st'):
+      (PRIV: a ∉ pub_actions)
+      (STEP: amTrans odd_AM st (a, Some ρ) st'):
       cur_odd st = cur_odd st' (* /\ Nat.even (cur_odd st) *);
 
     ρ__o: amRole odd_AM;
@@ -112,8 +120,8 @@ Record OddModel := {
       exists st', amTrans odd_AM st (pub_act (step_sync (cur_odd st)), Some ρ__o) st';
     odd_syncable st (ODD: Nat.even (cur_odd st)):
       exists st', amTrans odd_AM st (pub_act (step_sync (cur_odd st)), None) st';
-    odd_stutterable st (ODD: Nat.even (cur_odd st)):
-      exists st' a, amTrans odd_AM st (priv_act a, Some ρ__o) st';
+    odd_stutterable st (ODD: Nat.even (cur_odd st))    :
+      exists st' a, a ∉ pub_actions /\ amTrans odd_AM st (a, Some ρ__o) st';
 
     odd_step_lr_nonincr st st' a oρ
       (STEP: amTrans odd_AM st (a, oρ) st'):
@@ -126,7 +134,7 @@ Record OddModel := {
   (* TODO: ? replace with "private actions don't preempt the sync one forever" condition *)
     odd_pub_priv_disj (st__o: amSt odd_AM):
     (exists k st__o', amTrans _ st__o (pub_act $ step_sync k, Some ρ__o) st__o') ->
-    (exists a st__o', amTrans _ st__o (priv_act a, Some ρ__o) st__o') ->
+    (exists a st__o', a ∉ pub_actions /\ amTrans _ st__o (a, Some ρ__o) st__o') ->
     False;
 }.
 
@@ -137,7 +145,7 @@ Proof.
   destruct (even_or_odd (cur_even _ st__e)) as [E | O]. 
   - eexists. eapply @even_steppable. intuition.
   - ogeneralize * even_stutterable; eauto.
-    intros (?&?&?). eauto.
+    intros (?&?&?&?). eauto.
 Qed.
 
 Lemma ρ__o_always_live `{om: OddModel} st__o:
@@ -146,6 +154,6 @@ Proof.
   apply AM_live_roles_spec. 
   destruct (even_or_odd (cur_odd _ st__o)) as [E | O]. 
   - ogeneralize * odd_stutterable; eauto.
-    intros (?&?&?). eauto.
+    intros (?&?&?&?). eauto.
   - eexists. eapply @odd_steppable. intuition.
 Qed.
